Add Veritas.Memory interface file

Veritas.Memory.fst
@@ -3,161 +3,11 @@ module Veritas.Memory
 open FStar.BitVector
 open FStar.Classical
 open FStar.Seq
-open Veritas.SubSeq
+open Veritas.SeqAux
 
-(* address is a 256 bit value *)
-let addr_size = 256
-type addr = bv_t addr_size
 
-(*
- * Payload of an address is either Null, a special initial value,
- * or an integer (TODO: replace integer with something more general)
- *)
-type payload =
-  | Null: payload
-  | Value: v:int -> payload
-
-(* Memory operation is either a read or a write *)
-type memory_op =
-  (* Read operation reading a value v at address a *)
-  | Read: a:addr -> v:payload -> memory_op
-  (* Write operation writing a value v at address a *)
-  | Write: a:addr -> v:payload -> memory_op
-
-(* Return address of a memory operator *)
-let address_of (o: memory_op): Tot addr =
-  match o with
-  | Read a _ -> a
-  | Write a _ -> a
-
-(* Log is a sequence of memory operations *)
-type memory_op_log = seq memory_op
-
-(* type of an index into a log *)
-type log_index (l:memory_op_log) = seq_index l
-
-(* Address of log entry at position i *)
-let address_at_idx (l:memory_op_log) (i:log_index l): Tot addr =
-  address_of (index l i)
-
-(* Is an operation at index i a read op *)
-let is_read_op (l:memory_op_log) (i:log_index l): Tot bool =
-  Read? (index l i)
-
-(* For a read operation, return the read value *)
-let read_value (l:memory_op_log) (i:log_index l{is_read_op l i}): Tot payload =
-  Read?.v (index l i)
-
-(* Is an operation at index i a write op *)
-let is_write_op (l:memory_op_log) (i:log_index l): Tot bool =
-  Write? (index l i)
-
-(* For a write operation, return the written value *)
-let written_value (l:memory_op_log) (i:log_index l{is_write_op l i}): Tot payload =
-  Write?.v (index l i)
-
-(*
- * Our goal is to define a notion of read-write consistency
- * for a memory_op_log. We do so using a naive verifier
- * that materializes the entire memory and checks if every
- * read operation reads the current value of that address
- *)
-
-(* Memory: mapping from address to payload *)
-type memory = addr -> payload
-
-(* The state of the naive verifier as it processes the log *)
-(* TODO: Learn about noeq - this does not seem to compile without it *)
-noeq type naive_verifier_state =
-  | NFailed: naive_verifier_state
-  | NValid: m:memory -> naive_verifier_state
-
-(* apply function for memory *)
-let apply (m:memory) (o:memory_op{Write? o}): Tot memory =
-  let a = Write?.a o in
-  let v = Write?.v o in
-  fun a' -> if a' = a then v else m a'
-
-(* Naive verifier that verifies read-write consistency of a log given an initial memory *)
-let rec naive_verifier (m:memory) (l:memory_op_log): Tot naive_verifier_state
-  (decreases (length l)) =
-  let n = length l in
-  if n = 0 then NValid m
-  else
-    let l' = slice l 0 (n - 1) in
-    // Recursively verify prefix
-    let vs = naive_verifier m l' in
-    // Propagate prefix failures
-    if NFailed? vs then NFailed
-    else
-      let o = index l (n - 1) in
-      let m' = NValid?.m vs in
-      if Read? o then
-        // Check value read is value in memory 
-        if Read?.v o = m' (Read?.a o) then vs else NFailed
-      else
-        // Apply write changes
-        NValid (apply m' o)
-
-(* Initial state of memory - all addresses have Null *)
-let init_memory:memory = fun _ -> Null
-
-(*
- * read-write consistency starting from the initial state where all
- * addresses are initialized to Null
- *)
-let rw_consistent (l:memory_op_log): Tot bool = NValid? (naive_verifier init_memory l)
-
-(*
- * We next prove that a particular property of the log - every read 
- * corresponds to the most recent write - implies read write 
- * consistency as defined above
- *)
-
-(* is this a write to address a *)
-let is_write_to_addr (a:addr) (o:memory_op) = 
-  Write? o && Write?.a o = a
-
-(* 
- * last_write to an address a if it exists
- *)
-let last_write (l:memory_op_log) (a:addr):
-  Tot (option (i:(log_index l){is_write_to_addr a (index l i)})) =
-  let f = is_write_to_addr a in
-  let optwi = last_index l f in
-  if None? optwi then None
-  else
-    let wi = Some?.v optwi in
-    (last_index_correct1 l f; Some wi)
-
-(*
- * Given an index of the log, return the most recent previous write
- * to the address in the index if it exists
- *)
-let prev_write_of_idx (l:memory_op_log) (i:log_index l):
-  Tot (option (j:log_index l{j < i && address_at_idx l j = address_at_idx l i && is_write_op l j})) =
-  let l' = slice l 0 i in
-  let a = address_at_idx l i in
-  let optj = last_write l' a in
-  if None? optj then None
-  else
-    let j = Some?.v optj in
-    (
-      lemma_len_slice l 0 i;
-      lemma_index_slice l 0 i j;
-      Some j
-    )
-
-(*
- * Does an address have a write in a log?
- *)
-let has_some_write (l:memory_op_log) (a:addr): Tot bool =
-  Some? (last_write l a)
-
-(* Given an address with some write, return the value of the last write *)
 let last_write_value (l:memory_op_log) (a:addr{has_some_write l a}): Tot payload =
-  let i = Some?.v (last_write l a) in
-  written_value l i
+  written_value l (last_write_idx l a)
 
 (* 
  * If an address has a write, then the memory of the naive verifier 
@@ -169,14 +19,20 @@ let rec memory_is_last_write (l:memory_op_log) (m:memory) (a:addr):
         (decreases (length l)) =
   let n = length l in
   let f = is_write_to_addr a in
+  let li = last_write_idx l a in
   if n = 0 then ()
-  else 
+  else if f (index l (n - 1)) then 
+    if li = n - 1 then ()
+    else lemma_last_index_correct1 f l (n - 1)  
+  else if li = n - 1 then ()
+  else (
     let l' = prefix l (n - 1) in
-    if f (index l (n - 1)) then ()      
-    else (
-        memory_is_last_write l' m a;
-        last_index_prefix l f
-    )
+    lemma_prefix_index l (n - 1) li;
+    lemma_last_index_correct2 f l' li;
+    memory_is_last_write l' m a;    
+    lemma_last_index_correct1 f l (n - 1);
+    lemma_last_index_prefix f l (n - 1)
+  ) 
 
 (*
  * If we start with initial memory (all addresses null), then the 
@@ -190,60 +46,47 @@ let rec memory_is_null_without_write (l:memory_op_log) (a:addr):
   let n = length l in
   let f = is_write_to_addr a in
   if n = 0 then ()
-  else
-    let l' = slice l 0 (n - 1) in
-    if is_write_op l (n - 1) then
-      if address_at_idx l (n - 1) = a then
-        exists_implies_last_index l f (n - 1)
-      else
-        memory_is_null_without_write l' a
+  else if f (index l (n - 1)) then
+    lemma_last_index_correct2 f l (n - 1)
+  else (
+    let l' = prefix l (n - 1) in
+    if has_some_write l' a then (
+      lemma_prefix_index l (n - 1) (last_write_idx l' a);
+      lemma_last_index_correct2 f l (last_write_idx l' a)
+    )
     else
       memory_is_null_without_write l' a
+  )
 
-(* Has there been a previous write to address at index i *)
-let has_prev_write (l:memory_op_log) (i:log_index l): Tot bool =
-  Some? (prev_write_of_idx l i)
-
-(* not (has_prev_write) *)
-let has_no_prev_write (l:memory_op_log) (i:log_index l): Tot bool =
-  None? (prev_write_of_idx l i)
-
-(* 
- * If every read, reads the previous write, then we have read-write
- * consistency as defined by the naive verifier
- *)
-let rec read_last_write_implies_rwconsistent (l:memory_op_log):
-  Lemma (requires (forall (i:log_index l).
-                        is_read_op l i ==>
-                          has_no_prev_write l i && read_value l i = Null ||
-                          has_prev_write l i && read_value l i = written_value l (Some?.v (prev_write_of_idx l i))))
-       (ensures (rw_consistent l))
-       (decreases (length l))
-       =
+let rec lemma_rw_consistent_operational_correct_aux (l:rw_consistent_operational):
+  Lemma (requires (True))
+        (ensures (rw_consistent l))
+        (decreases (length l))
+  = 
   let n = length l in
   if n = 0 then ()
-  else
-    let l' = slice l 0 (n - 1) in
-    let o = index l (n - 1) in
+  else 
+    let l' = prefix l (n - 1) in
+    let o = index l (n - 1) in 
     let vs' = naive_verifier init_memory l' in
     let aux (i:log_index l'):
-      Lemma(is_read_op l' i ==>
-                       has_no_prev_write l' i && read_value l' i = Null ||
-                       has_prev_write l' i && read_value l' i = written_value l' (Some?.v (prev_write_of_idx l' i))) =
-      lemma_index_slice l 0 (n - 1) i;
-      if is_read_op l' i then
-        if has_no_prev_write l' i then
-          // TODO: Do asserts have side-effects? The proof
-          // goes through with the assert, but fails when the assert
-          // is commented out; some kind of forall_intro better here?
-          assert (has_no_prev_write l i)
+      Lemma(is_read_op l' i ==> 
+              read_value l' i = last_write_value_or_null (prefix l' i) (address_at_idx l' i)) = 
+      let pi = prefix l' i in
+      let a = address_at_idx l' i in
+      lemma_prefix_index l (n - 1) i;
+      lemma_prefix_prefix l (n - 1) i;
+      assert (pi = prefix l i);
+      if is_read_op l' i then 
+        if has_some_write (prefix l' i) (address_at_idx l' i) then 
+          assert (has_some_write (prefix l i) (address_at_idx l i))        
         else
-          assert (has_prev_write l i)        
+          assert (not (has_some_write (prefix l i) (address_at_idx l i)))      
       else ()
       in
-    forall_intro aux; read_last_write_implies_rwconsistent l';
+    forall_intro aux; lemma_rw_consistent_operational_correct_aux l';
     assert (NValid? vs');
-    let m' = (NValid?.m vs') in
+        let m' = (NValid?.m vs') in
     if Write? o then ()
     else
       let a = address_of o in
@@ -256,3 +99,7 @@ let rec read_last_write_implies_rwconsistent (l:memory_op_log):
         assert (is_read_op l (n - 1))
       )
 
+let lemma_rw_consistent_operational_correct (l:rw_consistent_operational):
+    Lemma (requires (True))
+        (ensures (rw_consistent l))
+        (decreases (length l)) = lemma_rw_consistent_operational_correct_aux l
