Veritas.SeqAux.fst
@@ -1,43 +1,58 @@
 module Veritas.SeqAux
 
+open FStar.Classical
 open FStar.Seq
 
 let prefix (#a:Type) (s:seq a) (i:nat{i <= length s}) = slice s 0 i
 
 let lemma_prefix_index (#a:Type) (s:seq a) (i:nat{i <= length s}) (j:nat{j < i}):
   Lemma (requires (True))
-        (ensures (index (prefix s i) j == index s j)) = 
+        (ensures (index (prefix s i) j == index s j)) =
   lemma_index_slice s 0 i j
 
-let suffix (#a:Type) (s:seq a) (i:nat{i <= length s}) = 
+let lemma_prefix_prefix (#a:Type) (s:seq a) (i:nat{i <= length s}) (j:nat{j <= i}):
+  Lemma (requires (True))
+        (ensures (prefix (prefix s i) j == prefix s j)) = 
+  let pij = prefix (prefix s i) j in
+  let pj = prefix s j in
+  let pi = prefix s i in
+  let aux (k:nat{k < j}):
+    Lemma (index pij k == index pj k) = 
+    lemma_prefix_index s j k;
+    lemma_prefix_index s i k;
+    lemma_prefix_index pi j k
+  in
+  forall_intro aux; lemma_eq_intro pij pj
+
+let suffix (#a:Type) (s:seq a) (i:nat{i <= length s}) =
   slice s (length s - i) (length s)
 
 let lemma_suffix_index (#a:Type) (s:seq a) (i:nat{i <= length s}) (j:nat{j < i}):
   Lemma (requires (True))
-        (ensures (index (suffix s i) j == index s (length s - i + j))) = 
+        (ensures (index (suffix s i) j == index s (length s - i + j))) =
   lemma_index_slice s (length s - i) (length s) j
 
-(* 
- * TODO: For some reason a direct recursive implementation of filter 
+(*
+ * TODO: For some reason a direct recursive implementation of filter
  * fails to compile
  *)
-let rec filter_aux (#a:eqtype) (f:a -> bool) (s:seq a) : Tot (seq a)  
-  (decreases (length s)) = 
+let rec filter_aux (#a:eqtype) (f:a -> bool) (s:seq a) : Tot (seq a)
+  (decreases (length s)) =
   let n = length s in
   if n = 0 then empty
-  else 
-    let e = index s (n - 1) in 
+  else
+    let e = index s (n - 1) in
     if f e then
-      append (filter_aux f (prefix s (n - 1))) (create 1 e)    
-    else 
+      append (filter_aux f (prefix s (n - 1))) (create 1 e)
+    else
       filter_aux f (prefix s (n - 1))
 
-let filter (#a:eqtype) (f:a -> bool) (s:seq a) : Tot (seq a)  = filter_aux f s 
+let filter (#a:eqtype) (f:a -> bool) (s:seq a) : Tot (seq a)  = filter_aux f s
 
 let rec filter_len_monotonic (#a:eqtype) (f:a -> bool) (s:seq a) (i:nat{i <= length s}):
   Lemma (requires (True))
         (ensures (length (filter f s) >= length (filter f (prefix s i))))
-        (decreases (length s)) = 
+        (decreases (length s)) =
   let n = length s in
   if n = 0 then ()
   else if i  = n then () // s == prefix s i
@@ -48,10 +63,10 @@ let rec filter_len_monotonic (#a:eqtype) (f:a -> bool) (s:seq a) (i:nat{i <= len
 
 let rank (#a:eqtype) (f:a -> bool)  (s:seq a) (i:nat{i <= length s})
   = length (filter f (prefix s i))
-        
-let filter_index_map_aux (#a:eqtype) (f:a -> bool)  (s:seq a) 
+
+let filter_index_map_aux (#a:eqtype) (f:a -> bool)  (s:seq a)
   (i:seq_index s{f (index s i)}):
-  Tot (seq_index (filter f s)) = 
+  Tot (seq_index (filter f s)) =
   filter_len_monotonic f s (i+1);
   lemma_len_append (filter f (prefix s i)) (create 1 (index s i));
   rank f s i
@@ -59,34 +74,34 @@ let filter_index_map_aux (#a:eqtype) (f:a -> bool)  (s:seq a)
 let rec filter_index_map_correct (#a:eqtype) (f:a -> bool) (s:seq a) (i:seq_index s):
   Lemma (requires (f (index s i)))
         (ensures (index s i = index (filter f s) (filter_index_map_aux f s i)))
-        (decreases (length s)) = 
+        (decreases (length s)) =
   let n = length s in
   if n = 0 then ()
   else if i = n - 1 then ()
   else filter_index_map_correct f (prefix s (n - 1)) i
 
 let filter_index_map (#a:eqtype) (f:a -> bool) (s:seq a) (i:seq_index s{f (index s i)}):
-  Tot (j:seq_index (filter f s){index s i = index (filter f s) j}) = 
+  Tot (j:seq_index (filter f s){index s i = index (filter f s) j}) =
   filter_index_map_correct f s i;
   filter_index_map_aux f s i
 
-let filter_index_map_monotonic (#a:eqtype) (f:a -> bool) (s:seq a)  
+let filter_index_map_monotonic (#a:eqtype) (f:a -> bool) (s:seq a)
   (i:seq_index s) (j:seq_index s{j > i}):
   Lemma (requires (f (index s i) && f (index s j)))
         (ensures (filter_index_map f s i < filter_index_map f s j)) =
   filter_len_monotonic f (prefix s j) (i + 1)
 
-let rank_increases_by_atmost_one (#a:eqtype) (f:a -> bool) (s:seq a) 
+let rank_increases_by_atmost_one (#a:eqtype) (f:a -> bool) (s:seq a)
   (i:seq_index s):
   Lemma (requires (True))
-        (ensures (f (index s i) && (rank f s i) + 1 = rank f s (i + 1) || 
+        (ensures (f (index s i) && (rank f s i) + 1 = rank f s (i + 1) ||
                   not (f (index s i)) && rank f s i = rank f s (i + 1))) = ()
 
-let rec rank_search (#a:eqtype) (f:a -> bool) (s:seq a) 
-                (r:seq_index (filter f s)) 
+let rec rank_search (#a:eqtype) (f:a -> bool) (s:seq a)
+                (r:seq_index (filter f s))
                 (i:nat{i <= length s && rank f s i > r})
   : Tot (j:seq_index s{rank f s j = r && f (index s j)})
-    (decreases i) = 
+    (decreases i) =
   assert (i > 0);
   if rank f s (i - 1) = r then (i - 1)
   else (
@@ -95,41 +110,50 @@ let rec rank_search (#a:eqtype) (f:a -> bool) (s:seq a)
   )
 
 let filter_index_inv_map (#a:eqtype) (f:a -> bool)  (s:seq a) (i:seq_index (filter f s))
-  : Tot (j:seq_index s{f (index s j) && filter_index_map f s j = i}) = 
+  : Tot (j:seq_index s{f (index s j) && filter_index_map f s j = i}) =
   rank_search f s i (length s)
 
 let last_index_opt (#a:eqtype) (f:a -> bool) (s:seq a):
-  Tot (option (i:seq_index s{f (index s i)})) = 
+  Tot (option (i:seq_index s{f (index s i)})) =
   let fs = filter f s in
   if length fs = 0 then None
   else Some (filter_index_inv_map f s ((length fs) - 1))
 
 let lemma_last_index_correct1 (#a:eqtype) (f:a -> bool) (s:seq a) (i:seq_index s):
   Lemma (requires (exists_sat_elems f s /\ i > last_index f s))
-        (ensures (not (f (index s i)))) = 
+        (ensures (not (f (index s i)))) =
   let j = last_index f s in
   if f (index s i) then
     filter_index_map_monotonic f s j i
-  else ()    
+  else ()
 
 let lemma_last_index_correct2 (#a:eqtype) (f:a -> bool)  (s:seq a) (i:seq_index s):
   Lemma (requires (f (index s i)))
-        (ensures (exists_sat_elems f s /\ last_index f s >= i)) = 
+        (ensures (exists_sat_elems f s /\ last_index f s >= i)) =
   let n = length s in
   let ri = filter_index_map f s i in
   assert (exists_sat_elems f s);
   let j = last_index f s in
-  if j < i then 
+  if j < i then
     filter_index_map_monotonic f s j i
   else ()
 
-let lemma_last_index_prefix (#a:eqtype) (f:a -> bool) (s:seq a):
-  Lemma (requires (exists_sat_elems f s))
-        (ensures (exists_sat_elems f (prefix s ((last_index f s) + 1)) /\
-                  last_index f s = last_index f (prefix s ((last_index f s) + 1)))) = 
-  let li = last_index f s in 
-  let s' = prefix s (li + 1) in
-  lemma_prefix_index s (li + 1) li;
+let lemma_last_index_prefix (#a:eqtype) (f:a -> bool) (s:seq a) (i:nat{i <= length s}):
+  Lemma (requires (exists_sat_elems f s /\ i > last_index f s))
+        (ensures (exists_sat_elems f (prefix s i) /\
+                  last_index f s = last_index f (prefix s i))) =
+  let li = last_index f s in
+  let s' = prefix s i in
+  lemma_prefix_index s i li;
+  assert(f (index s' li));
+  assert(li < length s');
   let r' = filter_index_map f s' li in
-  ()
-
+  assert(exists_sat_elems f s');
+  let li' = last_index f s' in
+  if li < li' then (
+    lemma_prefix_index s i li';
+    lemma_last_index_correct1 f s li'
+  )
+  else if li > li' then
+    lemma_last_index_correct1 f s' li
+  else ()
