Veritas.Memory.fsti
@@ -1,0 +1,144 @@
+module Veritas.Memory
+
+open FStar.BitVector
+open FStar.Seq
+open Veritas.SeqAux
+
+(* address is a 256 bit value *)
+let addr_size = 256
+type addr = bv_t addr_size
+
+(*
+ * Payload of an address is either Null, a special initial value,
+ * or an integer (TODO: replace integer with something more general)
+ *)
+type payload =
+  | Null: payload
+  | Value: v:int -> payload
+
+(* Memory operation is either a read or a write *)
+type memory_op =
+  (* Read operation reading a value v at address a *)
+  | Read: a:addr -> v:payload -> memory_op
+  (* Write operation writing a value v at address a *)
+  | Write: a:addr -> v:payload -> memory_op
+
+(* Return address of a memory operator *)
+let address_of (o: memory_op): Tot addr =
+  match o with
+  | Read a _ -> a
+  | Write a _ -> a
+
+(* Log is a sequence of memory operations *)
+type memory_op_log = seq memory_op
+
+(* type of an index into a log *)
+type log_index (l:memory_op_log) = seq_index l
+
+(* Address of log entry at position i *)
+let address_at_idx (l:memory_op_log) (i:log_index l): Tot addr =
+  address_of (index l i)
+
+(* Is an operation at index i a read op *)
+let is_read_op (l:memory_op_log) (i:log_index l): Tot bool =
+  Read? (index l i)
+
+(* For a read operation, return the read value *)
+let read_value (l:memory_op_log) (i:log_index l{is_read_op l i}): Tot payload =
+  Read?.v (index l i)
+
+(* Is an operation at index i a write op *)
+let is_write_op (l:memory_op_log) (i:log_index l): Tot bool =
+  Write? (index l i)
+
+(* For a write operation, return the written value *)
+let written_value (l:memory_op_log) (i:log_index l{is_write_op l i}): Tot payload =
+  Write?.v (index l i)
+
+(*
+ * Our goal is to define a notion of read-write consistency
+ * for a memory_op_log. We do so using a naive verifier
+ * that materializes the entire memory and checks if every
+ * read operation reads the current value of that address
+ *)
+
+(* Memory: mapping from address to payload *)
+type memory = addr -> payload
+
+(* The state of the naive verifier as it processes the log *)
+(* TODO: Learn about noeq - this does not seem to compile without it *)
+noeq type naive_verifier_state =
+  | NFailed: naive_verifier_state
+  | NValid: m:memory -> naive_verifier_state
+
+(* apply function for memory *)
+let apply (m:memory) (o:memory_op{Write? o}): Tot memory =
+  let a = Write?.a o in
+  let v = Write?.v o in
+  fun a' -> if a' = a then v else m a'
+
+(* Naive verifier that verifies read-write consistency of a log given an initial memory *)
+let rec naive_verifier (m:memory) (l:memory_op_log): Tot naive_verifier_state
+  (decreases (length l)) =
+  let n = length l in
+  if n = 0 then NValid m
+  else
+    let l' = prefix l (n - 1) in
+    // Recursively verify prefix
+    let vs = naive_verifier m l' in
+    // Propagate prefix failures
+    if NFailed? vs then NFailed
+    else
+      let o = index l (n - 1) in
+      let m' = NValid?.m vs in
+      if Read? o then
+        // Check value read is value in memory 
+        if Read?.v o = m' (Read?.a o) then vs else NFailed
+      else
+        // Apply write changes
+        NValid (apply m' o)
+
+(* Initial state of memory - all addresses have Null *)
+let init_memory:memory = fun _ -> Null
+
+(*
+ * read-write consistency starting from the initial state where all
+ * addresses are initialized to Null
+ *)
+let rw_consistent (l:memory_op_log): Tot bool = NValid? (naive_verifier init_memory l)
+
+(*
+ * We next prove that a particular property of the log - every read 
+ * corresponds to the most recent write - implies read write 
+ * consistency as defined above
+ *)
+
+(* is this a write to address a *)
+let is_write_to_addr (a:addr) (o:memory_op) = 
+  Write? o && Write?.a o = a
+
+(* last write to address a in log if it exists *)
+let last_write_idxopt (l:memory_op_log) (a:addr) = last_index_opt (is_write_to_addr a) l
+
+(* does there exist some write to address a in log *)
+let has_some_write (l:memory_op_log) (a:addr) = exists_sat_elems (is_write_to_addr a) l
+
+(* index of last write to a if we know it exists *)
+let last_write_idx (l:memory_op_log) (a:addr{has_some_write l a}) = last_index (is_write_to_addr a) l
+
+(* last written value if exists or null *)
+let last_write_value_or_null (l:memory_op_log) (a:addr): Tot payload = 
+  if has_some_write l a then
+    written_value l (last_write_idx l a)
+  else
+    Null
+
+(* operational definition of read-write consistency *)
+type rw_consistent_operational = 
+  l:memory_op_log{forall (i:log_index l). 
+                    is_read_op l i ==> 
+                    read_value l i = last_write_value_or_null (prefix l i) (address_at_idx l i)}
+
+(* operational consistency implies rw_consistency based on naive verifier *)
+val lemma_rw_consistent_operational_correct (l:rw_consistent_operational):
+  Lemma (rw_consistent l)
